@prefix : <http://makolab.com/oc/> .
@prefix owl: <http://www.w3.org/2002/07/owl#> .
@prefix rdf: <http://www.w3.org/1999/02/22-rdf-syntax-ns#> .
@prefix xml: <http://www.w3.org/XML/1998/namespace> .
@prefix xsd: <http://www.w3.org/2001/XMLSchema#> .
@prefix rdfs: <http://www.w3.org/2000/01/rdf-schema#> .
@prefix skos: <http://www.w3.org/2004/02/skos/core#> .

<http://makolab.com/oc/> a owl:Ontology ;
	owl:versionInfo "varion 1.0"@en ;
	rdfs:comment """Created by MakoLab S.A.

Contact:
Robert Trypuz (robert.trypuz@makolab.pl)"""@en ;
	rdfs:label "Ontology of change with manifestations"@en .
# 
# 
# #################################################################
# #
# #    Annotation properties
# #
# #################################################################
# 
# 
# http://www.w3.org/2004/02/skos/core#definition

skos:definition a owl:AnnotationProperty .
# 
# http://www.w3.org/2004/02/skos/core#scopeNote

skos:scopeNote a owl:AnnotationProperty .
# 
# 
# 
# #################################################################
# #
# #    Object Properties
# #
# #################################################################
# 
# 
# http://makolab.com/oc/hasLastManifestation

:hasLastManifestation a owl:ObjectProperty ;
	rdfs:subPropertyOf :hasManifestation ;
	owl:inverseOf :isLastManifestationOf ;
	rdfs:label "has last manifestation"@en ;
	skos:definition "The property assigns the last manifestation to a variable entity."@en .
# 
# http://makolab.com/oc/hasManifestation

:hasManifestation a owl:ObjectProperty ;
	owl:inverseOf :isManifestationOf ;
	rdfs:domain :VariableEntity ;
	rdfs:range :VariableEntityManifestation ;
	rdfs:label "has manifestation"@en ;
	skos:definition "The property assigns a manifestation to a variable entity."@en .
# 
# http://makolab.com/oc/hasPredecessorEntityManifestation

:hasPredecessorEntityManifestation a owl:ObjectProperty ;
	owl:inverseOf :isPredecessorEntityManifestationOf ;
	rdfs:domain :VariableEntityManifestation ;
	rdfs:range :VariableEntityManifestation ;
	rdfs:label "has predecessor entity manifestation"@en ;
	skos:definition "The property establishes the temporal linear order of the manifestations of an entity."@en .
# 
# http://makolab.com/oc/hasSuccessorEntity

:hasSuccessorEntity a owl:ObjectProperty ;
	rdfs:domain :VariableEntityManifestation ;
	rdfs:range :VariableEntity ;
	rdfs:label "has successor entity"@en ;
	skos:definition "The property assigns to an entity other entity that supersedes or subsumes it."@en .
# 
# http://makolab.com/oc/isLastManifestationOf

:isLastManifestationOf a owl:ObjectProperty ;
	rdfs:subPropertyOf :isManifestationOf ;
	rdfs:label "is last manifestation of"@en ;
	skos:definition "The property indicates which manifestations of a variable entities are last."@en .
# 
# http://makolab.com/oc/isManifestationOf

:isManifestationOf a owl:ObjectProperty ;
	rdfs:domain :VariableEntityManifestation ;
	rdfs:range :VariableEntity ;
	rdfs:label "is manifestation of"@en ;
	skos:definition "The property indicates to each manifestation the variable entity it is a manifestation of."@en .
# 
# http://makolab.com/oc/isPredecessorEntityManifestationOf

:isPredecessorEntityManifestationOf a owl:ObjectProperty ;
	rdfs:domain :VariableEntityManifestation ;
	rdfs:range :VariableEntityManifestation ;
	rdfs:label "is predecessor entity manifestation of"@en ;
	skos:definition "The property establishes the temporal linear order of the manifestations of an entity."@en .
# 
# 
# 
# #################################################################
# #
# #    Data properties
# #
# #################################################################
# 
# 
# http://makolab.com/oc/hasBeginning

:hasBeginning a owl:DatatypeProperty ;
	rdfs:subPropertyOf :hasDate ;
	a owl:FunctionalProperty ;
	rdfs:domain :VariableEntityManifestation ;
	rdfs:range xsd:dateTime ;
	rdfs:label "has beginning"@en ;
	skos:definition "The property assigns to a variable entity manifestation date and time information about it was most recently updated."@en .
# 
# http://makolab.com/oc/hasDate

:hasDate a owl:DatatypeProperty ;
	rdfs:range xsd:dateTime ;
	rdfs:label "has date"@en .
# 
# http://makolab.com/oc/hasEnd

:hasEnd a owl:DatatypeProperty ;
	rdfs:subPropertyOf :hasDate ;
	a owl:FunctionalProperty ;
	rdfs:domain :VariableEntityManifestation ;
	rdfs:range xsd:dateTime ;
	rdfs:label "has end"@en ;
	skos:definition "The property assigns to a variable entity manifestation date and time information about it was most recently updated."@en .
# 
# http://makolab.com/oc/hasUpdateDate

:hasUpdateDate a owl:DatatypeProperty ;
	rdfs:subPropertyOf :hasDate ;
	a owl:FunctionalProperty ;
	rdfs:domain :VariableEntityManifestation ;
	rdfs:range xsd:dateTime ;
	rdfs:label "has update date"@en ;
	skos:definition "The property assigns to a variable entity manifestation date and time information about it was most recently updated."@en .
# 
# 
# 
# #################################################################
# #
# #    Classes
# #
# #################################################################
# 
# 
# http://makolab.com/oc/NonVariableEntity

:NonVariableEntity a owl:Class ;
	owl:disjointWith :VariableEntity ;
	rdfs:label "non-variable entity"@en ;
	skos:definition "Non-variable entities are entities that do not have different manifestations as different objects at different times and in different worlds or situations."@en .
# 
# http://makolab.com/oc/VariableEntity

:VariableEntity a owl:Class ;
	rdfs:subClassOf _:genid1 .

_:genid1 a owl:Restriction ;
	owl:onProperty :hasLastManifestation ;
	owl:someValuesFrom :VariableEntityManifestation .

:VariableEntity rdfs:label "variable entity"@en ;
	skos:definition "Variable entities are entities that have different manifestations as different objects at different times and in different worlds or situations. If a variable entity e is manifested at time t by some variable entity manifestation m, then e exists at t, takes a geographical location of m and has all qualities possessed by m in t. A variable entity possesses a quality q (without temporal reference) if all of its manifestations have this quality q."@en .
# 
# http://makolab.com/oc/VariableEntityManifestation

:VariableEntityManifestation a owl:Class ;
	rdfs:subClassOf :NonVariableEntity , _:genid2 .

_:genid2 a owl:Restriction ;
	owl:onProperty :isManifestationOf ;
	owl:qualifiedCardinality "1"^^xsd:nonNegativeInteger ;
	owl:onClass :VariableEntity .

:VariableEntityManifestation rdfs:subClassOf _:genid3 .

_:genid3 a owl:Restriction ;
	owl:onProperty :hasUpdateDate ;
	owl:someValuesFrom xsd:dateTime .

:VariableEntityManifestation rdfs:label "variable entity manifestation"@en ;
	skos:definition "A variable entity manifestation is a manifestation (in particular time and space with a particular collection of qualities) of a variable entity."@en .
# 
# Generated by the OWL API (version 4.2.5.20160517-0735) https://github.com/owlcs/owlapi
